theories/zoo_std/waiter_spsc__opaque.v
@@ -1,0 +1,6 @@
+Require Import zoo_std.waiter_spsc__code.
+
+#[global] Opaque waiter_spsc٠create.
+#[global] Opaque waiter_spsc٠notify.
+#[global] Opaque waiter_spsc٠try_wait.
+#[global] Opaque waiter_spsc٠wait.
